## P3.1
<br>
(a)  
$x(t)=[x_1(t),x_2(t)]$  
$x_1(t)=y(t)$  
$x_2(t)={dy(t) \over dt}$  
<br>
(b)    
$m{d^2y(t) \over dt^2}+b{dy(t) \over dt}+ky(t)=F(t)$  
$m{dx_2(t) \over dt}+bx_2(t)+kx_1(t)=F(t)$  
${dx_2(t) \over dt}=-{b \over m}x_2(t)-{k \over m}x_1(t)+{1 \over m}F(t)$  
<br>
(c)  

$\dot{x}$=$\begin{bmatrix}0&1\\-{k \over m}&-{b \over m}\\ \end{bmatrix}$$x(t)$+$\begin{bmatrix}0\\{1 \over m}\\ \end{bmatrix}$$F(t)$  
<br>
## P3.3
<br>
$L{di_L \over dt}=v_1(t)-(v_2(t)-v_c(t))$  
$\dot{x_1}={1 \over L}x_2+v_1(t)-v_2(t)$  
<br>
$-C{dv_c \over dt}=i_L(t)-{v_2(t)-v_c(t) \over R}$  
$\dot{x_2}=-{1 \over C}x_1-{1 \over RC}x_2-{1 \over R}v_2(t)$  
<br>
$v(t)=[v_1(t),v_2(t)]$  
$\dot{x}(t)=\begin{bmatrix}0&{1 \over L}\\-{1 \over C}&-{1 \over RC}\\ \end{bmatrix}x(t)+\begin{bmatrix}1&-1\\0&-{1 \over R}\\ \end{bmatrix}v(t)$  
<br>
## P3.5
(a)  
$H(s)={s+2 \over s(s+8)(s-3)}$  
$T(s)={Y(s) \over R(s)}={H(s) \over 1+H(s)}$  
$={s+2 \over s^3+5s^2-23s+2}$  
$={s^{-2}+2s^{-3} \over 1+5s^{-1}-23s^{-2}+2s^{-3}}$  
<br>
(b)  
$\dot{x}(t)=\begin{bmatrix}0&1&0\\0&0&1\\-2&23&-5\\ \end{bmatrix}x(t)+\begin{bmatrix}0\\0\\1\\ \end{bmatrix}u(t)$  
$y(t)=\begin{bmatrix}2&1&0\\ \end{bmatrix}x(t)$  
<br>
## P3.12
(a)  
$T(s)={8s+40 \over s^3+12s^2+44s+48}$  
$T(s)={8s^{-2}+40s^{-3} \over 1+12s^{-1}+44s^{-2}+48^{-3}}$  
$\dot{x}(t)=\begin{bmatrix}0&1&0\\0&0&1\\-48&-44&-12\\ \end{bmatrix}x(t)+\begin{bmatrix}0\\0\\1\\ \end{bmatrix}u(t)$  
$y(t)=\begin{bmatrix}40&8&0\\ \end{bmatrix}x(t)$  
<br>
(b)  
$\phi(t)=\mathcal{L}^{-1} \{(sI-A)^{-1}\}$  
$\begin{bmatrix}3e^{-2t} - 3e^{-4t} + e^{-6}&5e^{-2t}/4 - 2e^{-4t} + 3e^{-6}/4&e^{-2t}/8 - e^{-4t}/4 + e^{-6}/8\\
 12e^{-4t} - 6e^{-2t} - 6e^{-6t}& 8e^{-4t} - (5e^{-2t})/2 - (9e^{-6t})/2&   e^{-4t} - e^{-2t}/4 - (3e^{-6t)}/4\\
12e^{-2t} - 48e^{-4t} + 36e^{-6t}& 5e^{-2t} - 32e^{-4t} + 27e^{-6t}& e^{-2t}/2 - 4e^{-4t} + (9e^{-6t})/2\\ \end{bmatrix}$  
<br>
##P3.17
$\dot{x}(t)=\begin{bmatrix}1&1&-1\\4&3&0\\-2&13&10\\ \end{bmatrix}x(t)+\begin{bmatrix}0\\0\\4\\ \end{bmatrix}u(t)$  
$y(t)=\begin{bmatrix}1&0&0\\ \end{bmatrix}x(t)$    
$A=\begin{bmatrix}1&1&-1\\4&3&0\\-2&13&10\\ \end{bmatrix} \quad B=\begin{bmatrix}0\\0\\4\\ \end{bmatrix}$  
$C=\begin{bmatrix}1&0&0\\ \end{bmatrix} \quad D=0$  
$\phi(s)=(sI-A)^{-1}$  
$G(s)=C\phi B+D$  
$G(s)={-4(s - 3) \over s^3 - 14s^2 + 37s + 20}$

