{"nbformat":4,"nbformat_minor":0,"metadata":{"colab":{"provenance":[],"mount_file_id":"1fTekEBmFc0PeZYJ9spIRukMQYH1x7YPu","authorship_tag":"ABX9TyN90CPlB0K2oN6Nmk4q55/C"},"kernelspec":{"name":"python3","display_name":"Python 3"},"language_info":{"name":"python"}},"cells":[{"cell_type":"markdown","source":["## P3.1\n","<br>\n","(a)  \n","$x(t)=[x_1(t),x_2(t)]$  \n","$x_1(t)=y(t)$  \n","$x_2(t)={dy(t) \\over dt}$  \n","<br>\n","(b)    \n","$m{d^2y(t) \\over dt^2}+b{dy(t) \\over dt}+ky(t)=F(t)$  \n","$m{dx_2(t) \\over dt}+bx_2(t)+kx_1(t)=F(t)$  \n","${dx_2(t) \\over dt}=-{b \\over m}x_2(t)-{k \\over m}x_1(t)+{1 \\over m}F(t)$  \n","<br>\n","(c)  \n","\n","$\\dot{x}$=$\\begin{bmatrix}0&1\\\\-{k \\over m}&-{b \\over m}\\\\ \\end{bmatrix}$$x(t)$+$\\begin{bmatrix}0\\\\{1 \\over m}\\\\ \\end{bmatrix}$$F(t)$  \n","<br>\n","## P3.3\n","<br>\n","$L{di_L \\over dt}=v_1(t)-(v_2(t)-v_c(t))$  \n","$\\dot{x_1}={1 \\over L}x_2+v_1(t)-v_2(t)$  \n","<br>\n","$-C{dv_c \\over dt}=i_L(t)-{v_2(t)-v_c(t) \\over R}$  \n","$\\dot{x_2}=-{1 \\over C}x_1-{1 \\over RC}x_2-{1 \\over R}v_2(t)$  \n","<br>\n","$v(t)=[v_1(t),v_2(t)]$  \n","$\\dot{x}(t)=\\begin{bmatrix}0&{1 \\over L}\\\\-{1 \\over C}&-{1 \\over RC}\\\\ \\end{bmatrix}x(t)+\\begin{bmatrix}1&-1\\\\0&-{1 \\over R}\\\\ \\end{bmatrix}v(t)$  \n","<br>\n","## P3.5\n","(a)  \n","$H(s)={s+2 \\over s(s+8)(s-3)}$  \n","$T(s)={Y(s) \\over R(s)}={H(s) \\over 1+H(s)}$  \n","$={s+2 \\over s^3+5s^2-23s+2}$  \n","$={s^{-2}+2s^{-3} \\over 1+5s^{-1}-23s^{-2}+2s^{-3}}$  \n","<br>\n","(b)  \n","$\\dot{x}(t)=\\begin{bmatrix}0&1&0\\\\0&0&1\\\\-2&23&-5\\\\ \\end{bmatrix}x(t)+\\begin{bmatrix}0\\\\0\\\\1\\\\ \\end{bmatrix}u(t)$  \n","$y(t)=\\begin{bmatrix}2&1&0\\\\ \\end{bmatrix}x(t)$  \n","<br>\n","## P3.12\n","(a)  \n","$T(s)={8s+40 \\over s^3+12s^2+44s+48}$  \n","$T(s)={8s^{-2}+40s^{-3} \\over 1+12s^{-1}+44s^{-2}+48^{-3}}$  \n","$\\dot{x}(t)=\\begin{bmatrix}0&1&0\\\\0&0&1\\\\-48&-44&-12\\\\ \\end{bmatrix}x(t)+\\begin{bmatrix}0\\\\0\\\\1\\\\ \\end{bmatrix}u(t)$  \n","$y(t)=\\begin{bmatrix}40&8&0\\\\ \\end{bmatrix}x(t)$  \n","<br>\n","(b)  \n","$\\phi(t)=\\mathcal{L}^{-1} \\{(sI-A)^{-1}\\}$  \n","$\\begin{bmatrix}3e^{-2t} - 3e^{-4t} + e^{-6}&5e^{-2t}/4 - 2e^{-4t} + 3e^{-6}/4&e^{-2t}/8 - e^{-4t}/4 + e^{-6}/8\\\\\n"," 12e^{-4t} - 6e^{-2t} - 6e^{-6t}& 8e^{-4t} - (5e^{-2t})/2 - (9e^{-6t})/2&   e^{-4t} - e^{-2t}/4 - (3e^{-6t)}/4\\\\\n","12e^{-2t} - 48e^{-4t} + 36e^{-6t}& 5e^{-2t} - 32e^{-4t} + 27e^{-6t}& e^{-2t}/2 - 4e^{-4t} + (9e^{-6t})/2\\\\ \\end{bmatrix}$  \n","<br>\n","##P3.17\n","$\\dot{x}(t)=\\begin{bmatrix}1&1&-1\\\\4&3&0\\\\-2&13&10\\\\ \\end{bmatrix}x(t)+\\begin{bmatrix}0\\\\0\\\\4\\\\ \\end{bmatrix}u(t)$  \n","$y(t)=\\begin{bmatrix}1&0&0\\\\ \\end{bmatrix}x(t)$    \n","$A=\\begin{bmatrix}1&1&-1\\\\4&3&0\\\\-2&13&10\\\\ \\end{bmatrix} \\quad B=\\begin{bmatrix}0\\\\0\\\\4\\\\ \\end{bmatrix}$  \n","$C=\\begin{bmatrix}1&0&0\\\\ \\end{bmatrix} \\quad D=0$  \n","$\\phi(s)=(sI-A)^{-1}$  \n","$G(s)=C\\phi B+D$  \n","$G(s)={-4(s - 3) \\over s^3 - 14s^2 + 37s + 20}$\n",""],"metadata":{"id":"9yOWrMrOIDFP"}}]}